fix sep log definition

SeparationLogic.thy
@@ -10,18 +10,51 @@ datatype expr =
 | UnOpE unop expr
 | BinOpE binop expr expr
 
+fun e_size :: "expr \<Rightarrow> nat" where
+  "e_size (ConstE k) = length k"
+| "e_size (VarE v) = size v"
+| "e_size (Base _) = loc_N_B"
+| "e_size (Ende _) = loc_N_B"
+| "e_size (UnOpE _ e) = e_size e"
+| "e_size (BinOpE _ e _) = e_size e"
+
+fun expr_semantics :: "stack \<Rightarrow> blocks \<Rightarrow> expr \<Rightarrow> val" where
+  "expr_semantics S B (ConstE k) = k"
+| "expr_semantics S B (VarE x) = lookup S x"
+| "expr_semantics S B (Base e) = loc64_ops.to_val (base B (loc64_ops.from_val (expr_semantics S B e)))"
+| "expr_semantics S B (Ende e)= loc64_ops.to_val (ende B (loc64_ops.from_val (expr_semantics S B e)))"
+| "expr_semantics S B (UnOpE op e) = apply_unop op (expr_semantics S B e)"
+| "expr_semantics S B (BinOpE op e1 e2) = apply_binop op (expr_semantics S B e1) (expr_semantics S B e2)"
+
 datatype form =
   PointsTo expr expr (infix "\<mapsto>\<^sub>s" 60)
 | PointsToK expr byte expr ("_\<mapsto>\<^sub>_[_]")
 | PointsToTop expr expr ("_\<mapsto>\<top>[_]")
 | SepConj form form (infixl "\<^emph>" 50)
 | Disj form form (infixl "\<or>\<^sub>s" 55)
-| LinkedList "expr \<Rightarrow> expr \<Rightarrow> form" expr expr
-| DoublyLinkedList "expr \<Rightarrow> expr \<Rightarrow> expr \<Rightarrow> form" expr expr expr expr
+| LinkedList expr expr
+| DoublyLinkedList expr expr expr expr
 | Emp
 | TrueF
 | Atom condition expr expr
 | Exists var form
+
+fun is_symbolic_heap :: "form \<Rightarrow> bool" where
+  "is_symbolic_heap (SepConj f1 f2) = (is_symbolic_heap f1 \<and> is_symbolic_heap f2)"
+| "is_symbolic_heap (Disj _ _) = False"
+| "is_symbolic_heap (Exists _ f) = is_symbolic_heap f"
+| "is_symbolic_heap _ = True"
+
+fun quantifier_free :: "form \<Rightarrow> bool" where
+  "quantifier_free (SepConj f1 f2) = (quantifier_free f1 \<and> quantifier_free f2)"
+| "quantifier_free (Disj f1 f2) = (quantifier_free f1 \<and> quantifier_free f2)"
+| "quantifier_free (Exists _ f) = False"
+| "quantifier_free _ = True"
+
+fun pure :: "form \<Rightarrow> bool" where
+  "pure (SepConj f1 f2) = (pure f1 \<and> pure f2)"
+| "pure (Atom _ _ _) = True"
+| "pure _ = False"
 
 class frees =
   fixes free_vars :: "'a \<Rightarrow> var set"
@@ -43,8 +76,8 @@ fun free_vars_form :: "form \<Rightarrow> var set" where
 | "free_vars_form (PointsToTop e1 e2) = free_vars e1 \<union> free_vars e2"
 | "free_vars_form (SepConj f1 f2) = free_vars_form f1 \<union> free_vars_form f2"
 | "free_vars_form (Disj f1 f2) = free_vars_form f1 \<union> free_vars_form f2"
-| "free_vars_form (LinkedList _ e1 e2) = free_vars e1 \<union> free_vars e2"
-| "free_vars_form (DoublyLinkedList _ e1 e2 e3 e4) = free_vars e1 \<union> free_vars e2 \<union> free_vars e3 
+| "free_vars_form (LinkedList e1 e2) = free_vars e1 \<union> free_vars e2"
+| "free_vars_form (DoublyLinkedList e1 e2 e3 e4) = free_vars e1 \<union> free_vars e2 \<union> free_vars e3 
   \<union> free_vars e4"
 | "free_vars_form Emp = {}"
 | "free_vars_form TrueF = {}"
@@ -52,44 +85,47 @@ fun free_vars_form :: "form \<Rightarrow> var set" where
 | "free_vars_form (Exists v f) = free_vars_form f - {v}"
 instance .. end
 
-fun e_size :: "expr \<Rightarrow> nat" where
-  "e_size (ConstE k) = length k"
-| "e_size (VarE v) = size v"
-| "e_size (Base _) = loc_N_B"
-| "e_size (Ende _) = loc_N_B"
-| "e_size (UnOpE _ e) = e_size e"
-| "e_size (BinOpE _ e _) = e_size e"
+abbreviation pointsto_sem :: "expr \<Rightarrow> expr \<Rightarrow> pre_config \<Rightarrow> bool" where
+  "pointsto_sem e1 e2 c \<equiv> case c of (S,B,M) \<Rightarrow> 
+    (dom M = {x. loc64_ops.from_val (expr_semantics S B e1) \<le> x \<and> 
+    x < offset (loc64_ops.from_val (expr_semantics S B e1)) (e_size e2)} \<and>
+    access M (loc64_ops.from_val (expr_semantics S B e1)) (e_size e2) = Some (expr_semantics S B e2))"
 
-fun is_symbolic_heap :: "form \<Rightarrow> bool" where
-  "is_symbolic_heap (SepConj f1 f2) = (is_symbolic_heap f1 \<and> is_symbolic_heap f2)"
-| "is_symbolic_heap (Disj _ _) = False"
-| "is_symbolic_heap (Exists _ f) = is_symbolic_heap f"
-| "is_symbolic_heap _ = True"
+text \<open>We need form to be deeply embedded so that we can talk about symbolic heaps and 
+  quantifier free formulae. We also need \<Lambda> to return a form so that we can restrict it 
+  to symbolic heaps in prenex form. But because \<Lambda> can potentially make the logic's semantics 
+  non-terminating, we can't define them over a completely deeply embedded form with \<Lambda>.\<close>
 
-fun quantifier_free :: "form \<Rightarrow> bool" where
-  "quantifier_free (SepConj f1 f2) = (quantifier_free f1 \<and> quantifier_free f2)"
-| "quantifier_free (Disj f1 f2) = (quantifier_free f1 \<and> quantifier_free f2)"
-| "quantifier_free (Exists _ f) = False"
-| "quantifier_free _ = True"
+locale separation_logic =
+  fixes \<Lambda> :: "(expr \<Rightarrow> expr \<Rightarrow> form) \<times> (expr \<Rightarrow> expr \<Rightarrow> pre_config \<Rightarrow> bool)"
+    and d\<Lambda> :: "(expr \<Rightarrow> expr \<Rightarrow> expr \<Rightarrow> form) \<times> (expr \<Rightarrow> expr \<Rightarrow> expr \<Rightarrow> pre_config \<Rightarrow> bool)"
+begin
 
-fun pure :: "form \<Rightarrow> bool" where
-  "pure (SepConj f1 f2) = (pure f1 \<and> pure f2)"
-| "pure (Atom _ _ _) = True"
-| "pure _ = False"
-
-fun expr_semantics :: "stack \<Rightarrow> blocks \<Rightarrow> expr \<Rightarrow> val" where
-  "expr_semantics S B (ConstE k) = k"
-| "expr_semantics S B (VarE x) = lookup S x"
-| "expr_semantics S B (Base e) = loc64_ops.to_val (base B (loc64_ops.from_val (expr_semantics S B e)))"
-| "expr_semantics S B (Ende e)= loc64_ops.to_val (ende B (loc64_ops.from_val (expr_semantics S B e)))"
-| "expr_semantics S B (UnOpE op e) = apply_unop op (expr_semantics S B e)"
-| "expr_semantics S B (BinOpE op e1 e2) = apply_binop op (expr_semantics S B e1) (expr_semantics S B e2)"
+inductive list_semantics :: "pre_config \<Rightarrow> form \<Rightarrow> bool" where
+  \<comment> \<open>Either the list is empty...\<close>
+  "\<lbrakk>M = Map.empty; eval_cond Eq (expr_semantics S B e1) (expr_semantics S B e2)\<rbrakk>
+  \<Longrightarrow> list_semantics (S,B,M) (LinkedList e1 e2)"
+  \<comment> \<open>... or we can take one segment and get its semantics from \<Lambda>.\<close>
+| "\<lbrakk>eval_cond Neq (expr_semantics S B e1) (expr_semantics S B e2); 
+    \<comment> \<open>For this get new variable and location denoting the second element and split of a heap for \<Lambda>\<close>
+    u \<notin> free_vars e1 \<union> free_vars e2; dom M1 \<inter> dom M2 = {}; M = M1 ++ M2; 
+    snd \<Lambda> e1 (VarE u) (update_stack S u (loc64_ops.to_val l),B,M1);
+    list_semantics (update_stack S u (loc64_ops.to_val l),B,M2) (LinkedList (VarE u) e2)\<rbrakk>
+   \<Longrightarrow> list_semantics (S,B,M) (LinkedList e1 e2)"
+  \<comment> \<open>And the same for doubly-linked lists.\<close>
+| "\<lbrakk>M = Map.empty; eval_cond Eq (expr_semantics S B e1) (expr_semantics S B e1');
+    eval_cond Eq (expr_semantics S B e2) (expr_semantics S B e2')\<rbrakk>
+  \<Longrightarrow> list_semantics (S,B,M) (DoublyLinkedList e1 e2 e1' e2')"
+| "\<lbrakk>eval_cond Neq (expr_semantics S B e1) (expr_semantics S B e1');
+    eval_cond Neq (expr_semantics S B e2) (expr_semantics S B e2');
+    u \<notin> free_vars e1 \<union> free_vars e2; om M1 \<inter> dom M2 = {}; M = M1 ++ M2;
+    snd d\<Lambda> e1 (VarE u) e2 (update_stack S u (loc64_ops.to_val l),B,M1);
+    list_semantics (update_stack S u (loc64_ops.to_val l),B,M2) (DoublyLinkedList (VarE u) e1 e1' e2')\<rbrakk>
+  \<Longrightarrow> list_semantics (S,B,M) (DoublyLinkedList e1 e2 e1' e2')"
 
 fun form_semantics :: "pre_config \<Rightarrow> form \<Rightarrow> bool" (infix "\<turnstile>" 80)
   where
-  "(S,B,M) \<turnstile> (e1 \<mapsto>\<^sub>s e2) = (dom M = {x. loc64_ops.from_val (expr_semantics S B e1) \<le> x \<and> 
-    x < offset (loc64_ops.from_val (expr_semantics S B e1)) (e_size e2)} \<and>
-    access M (loc64_ops.from_val (expr_semantics S B e1)) (e_size e2) = Some (expr_semantics S B e2))"
+  "(S,B,M) \<turnstile> (e1 \<mapsto>\<^sub>s e2) = pointsto_sem e1 e2 (S,B,M)"
 | "(S,B,M) \<turnstile> (e1 \<mapsto>\<^sub>k[e2]) = (dom M = {x. loc64_ops.from_val (expr_semantics S B e1) \<le> x \<and> 
     x < offset (loc64_ops.from_val (expr_semantics S B e1)) (e_size e2)} \<and> ran M = {k})"
 | "(S,B,M) \<turnstile> (e1 \<mapsto>\<top>[e2]) = (dom M = {x. loc64_ops.from_val (expr_semantics S B e1) \<le> x \<and> 
@@ -100,8 +136,27 @@ fun form_semantics :: "pre_config \<Rightarrow> form \<Rightarrow> bool" (infix 
 | "(S,B,M) \<turnstile> TrueF = True"
 | "(S,B,M) \<turnstile> (Atom cond e1 e2) = (M = Map.empty \<and> eval_cond cond (expr_semantics S B e1) (expr_semantics S B e2))"
 | "(S,B,M) \<turnstile> (Exists x f) = (\<exists>v. (update_stack S x v,B,M) \<turnstile> f)"
-| "(S,B,M) \<turnstile> (LinkedList \<Lambda> e1 e2) = ((S,B,M) \<turnstile> (Atom Eq e1 e2) \<or>
-   ((S,B,M) \<turnstile> ((Atom Neq e1 e2) \<^emph> TrueF) \<and> 
-    (\<exists>l u. u \<notin> free_vars e1 \<union> free_vars e2 \<and> 
-    (update_stack S u (loc64_ops.to_val l),B,M) \<turnstile> ((\<Lambda> e1 (VarE u)) \<^emph> (LinkedList \<Lambda> (VarE u) e2)))))"
+| "c \<turnstile> l = list_semantics c l"
+end
+
+locale sound_separation_logic = separation_logic
+  + assumes sound_lambda: "\<forall>c e1 e2. c \<turnstile> (fst \<Lambda> e1 e2) \<longleftrightarrow> snd \<Lambda> e1 e2 c"
+    and sound_dlambda: "\<forall>c e1 e2 e3. c \<turnstile> (fst d\<Lambda> e1 e2 e3) \<longleftrightarrow> snd d\<Lambda> e1 e2 e3 c"
+
+interpretation standard_sl: 
+  sound_separation_logic "((\<lambda>x y. x \<mapsto>\<^sub>s y), pointsto_sem)"
+    "((\<lambda>x y z. (x\<mapsto>\<^sub>sz) \<^emph> ((BinOpE plus x (ConstE [8]))\<mapsto>\<^sub>sy)), 
+      (\<lambda>x y z (S,B,M). \<exists>M1 M2. dom M1 \<inter> dom M2 = {} \<and> M = M1 ++ M2 \<and>
+      pointsto_sem x z (S,B,M1) \<and> pointsto_sem (BinOpE plus x (ConstE [8])) y (S,B,M2)))"
+proof (standard)
+  let ?\<Lambda> = "((\<lambda>x y. x \<mapsto>\<^sub>s y), pointsto_sem)"
+  let ?d\<Lambda> = "((\<lambda>x y z. (x\<mapsto>\<^sub>sz) \<^emph> ((BinOpE plus x (ConstE [8]))\<mapsto>\<^sub>sy)), 
+      (\<lambda>x y z (S,B,M). \<exists>M1 M2. dom M1 \<inter> dom M2 = {} \<and> M = M1 ++ M2 \<and>
+      pointsto_sem x z (S,B,M1) \<and> pointsto_sem (BinOpE plus x (ConstE [8])) y (S,B,M2)))"
+
+  show "\<forall>c e1 e2. separation_logic.form_semantics ?\<Lambda> ?d\<Lambda> c (fst ?\<Lambda> e1 e2)  \<longleftrightarrow> snd ?\<Lambda> e1 e2 c" sorry
+  show "\<forall>c e1 e2 e3. separation_logic.form_semantics ?\<Lambda> ?d\<Lambda> c (fst ?d\<Lambda> e1 e2 e3) \<longleftrightarrow> snd ?d\<Lambda> e1 e2 e3 c"
+    sorry
+qed
+
 end
